

# Worksheet 21

Parth Bhargava · A0310667E

**PC3261**  
**Classical Mechanics II**

November 21, 2025

## Problem 8.9

A simple pendulum of mass  $m$  and length  $\ell$  is subjected to a linear resistance force  $\mathbf{F} = -\gamma\mathbf{v}$  with  $\gamma > 0$ .

Obtain the equation of motion with suitable generalized coordinates.

### Solution

**Choose generalized coordinate:**

We use the angle  $\theta$  as the generalized coordinate, measured from the vertical downward direction.

**Position and velocity in Cartesian coordinates:**

$$\begin{cases} x = \ell \sin \theta & \Rightarrow \dot{x} = \ell \dot{\theta} \cos \theta \\ y = -\ell \cos \theta & \Rightarrow \dot{y} = \ell \dot{\theta} \sin \theta \end{cases}$$

**Lagrangian:**

The velocity is:

$$\begin{aligned} \mathbf{v} &= \dot{x}\hat{e}_x + \dot{y}\hat{e}_y = \ell\dot{\theta}\cos\theta\hat{e}_x + \ell\dot{\theta}\sin\theta\hat{e}_y \\ |\mathbf{v}|^2 &= \ell^2\dot{\theta}^2(\cos^2\theta + \sin^2\theta) = \ell^2\dot{\theta}^2 \end{aligned}$$

Kinetic energy:

$$T = \frac{m}{2} |\mathbf{v}|^2 = \frac{m}{2} \ell^2 \dot{\theta}^2$$

Potential energy:

$$U = mgy = -mg\ell \cos \theta$$

Lagrangian:

$$L(\theta, \dot{\theta}) = \frac{m}{2} \ell^2 \dot{\theta}^2 + mg\ell \cos \theta$$

**Resistance force:**

The resistance force is:

$$\mathbf{F}_{\text{res}} = -\gamma\mathbf{v} = -\gamma\ell\dot{\theta}\cos\theta\hat{e}_x - \gamma\ell\dot{\theta}\sin\theta\hat{e}_y$$

**Generalized force:**

The generalized force corresponding to  $\theta$  is:

$$\mathcal{Q}_\theta = \mathbf{F}_{\text{res}} \cdot \frac{\partial \mathbf{r}}{\partial \theta}$$

where:

$$\frac{\partial \mathbf{r}}{\partial \theta} = \frac{\partial}{\partial \theta} (x \hat{e}_x + y \hat{e}_y) = \ell \cos \theta \hat{e}_x + \ell \sin \theta \hat{e}_y$$

Therefore:

$$\begin{aligned} \mathcal{Q}_\theta &= (-\gamma \ell \dot{\theta} \cos \theta \hat{e}_x - \gamma \ell \dot{\theta} \sin \theta \hat{e}_y) \cdot (\ell \cos \theta \hat{e}_x + \ell \sin \theta \hat{e}_y) \\ &= -\gamma \ell \dot{\theta} \cos \theta \cdot \ell \cos \theta - \gamma \ell \dot{\theta} \sin \theta \cdot \ell \sin \theta \\ &= -\gamma \ell^2 \dot{\theta} (\cos^2 \theta + \sin^2 \theta) \\ &= -\gamma \ell^2 \dot{\theta} \end{aligned}$$

**Euler-Lagrange equation with non-conservative force:**

$$\frac{d}{dt} \left( \frac{\partial L}{\partial \dot{\theta}} \right) - \frac{\partial L}{\partial \theta} = \mathcal{Q}_\theta$$

Computing the partial derivatives:

$$\begin{cases} \frac{\partial L}{\partial \dot{\theta}} = m \ell^2 \dot{\theta} \\ \frac{\partial L}{\partial \theta} = -m g \ell \sin \theta \end{cases}$$

The equation becomes:

$$\begin{aligned} m \ell^2 \ddot{\theta} - (-m g \ell \sin \theta) &= -\gamma \ell^2 \dot{\theta} \\ m \ell^2 \ddot{\theta} + m g \ell \sin \theta &= -\gamma \ell^2 \dot{\theta} \end{aligned}$$

Dividing by  $m \ell^2$ :

$$\ddot{\theta} + \frac{\gamma}{m} \dot{\theta} + \frac{g}{\ell} \sin \theta = 0$$

This is the equation of motion for a damped pendulum.

**For small angles** ( $\sin \theta \approx \theta$ ):

$$\ddot{\theta} + \frac{\gamma}{m} \dot{\theta} + \frac{g}{\ell} \theta \approx 0$$

This is the equation for a damped harmonic oscillator with:

- Damping coefficient:  $\gamma/m$
- Natural frequency:  $\omega_0 = \sqrt{g/\ell}$

**Problem 8.10**

Show that the Galilean transformation is a gauge transformation for the Lagrangian of a system of  $N$  particles interacting via central potentials. Identify the gauge function.

**Lagrangian:**

$$L(\{\mathbf{r}_\alpha, \dot{\mathbf{r}}_\alpha\}) = \sum_{\alpha=1}^N \frac{m_\alpha}{2} \dot{\mathbf{r}}_\alpha \cdot \dot{\mathbf{r}}_\alpha - \frac{1}{2} \sum_{\alpha=1}^N \sum_{\beta \neq \alpha}^N U_{\alpha\beta}(|\mathbf{r}_\alpha - \mathbf{r}_\beta|)$$

**Galilean transformation:**

$$\mathbf{r}_\alpha(t) \rightarrow \mathbf{r}'_\alpha(t) = \mathbf{r}_\alpha(t) + \mathbf{V}t$$

**Solution**

**Transform the velocities:**

Under the Galilean transformation:

$$\mathbf{r}'_\alpha(t) = \mathbf{r}_\alpha(t) + \mathbf{V}t$$

Taking the time derivative:

$$\dot{\mathbf{r}}'_\alpha(t) = \dot{\mathbf{r}}_\alpha(t) + \mathbf{V}$$

**Transform the kinetic energy:**

$$\begin{aligned} T' &= \sum_{\alpha=1}^N \frac{m_\alpha}{2} \dot{\mathbf{r}}'_\alpha \cdot \dot{\mathbf{r}}'_\alpha \\ &= \sum_{\alpha=1}^N \frac{m_\alpha}{2} (\dot{\mathbf{r}}_\alpha + \mathbf{V}) \cdot (\dot{\mathbf{r}}_\alpha + \mathbf{V}) \\ &= \sum_{\alpha=1}^N \frac{m_\alpha}{2} [\dot{\mathbf{r}}_\alpha \cdot \dot{\mathbf{r}}_\alpha + 2\dot{\mathbf{r}}_\alpha \cdot \mathbf{V} + \mathbf{V} \cdot \mathbf{V}] \\ &= \sum_{\alpha=1}^N \frac{m_\alpha}{2} \dot{\mathbf{r}}_\alpha \cdot \dot{\mathbf{r}}_\alpha + \sum_{\alpha=1}^N m_\alpha \dot{\mathbf{r}}_\alpha \cdot \mathbf{V} + \sum_{\alpha=1}^N \frac{m_\alpha}{2} \mathbf{V} \cdot \mathbf{V} \end{aligned}$$

**Transform the potential energy:**

The potential depends only on relative positions:

$$|\mathbf{r}'_\alpha - \mathbf{r}'_\beta| = |(\mathbf{r}_\alpha + \mathbf{V}t) - (\mathbf{r}_\beta + \mathbf{V}t)| = |\mathbf{r}_\alpha - \mathbf{r}_\beta|$$

Therefore, the potential energy is unchanged:

$$U'(\{\mathbf{r}'_\alpha\}) = U(\{\mathbf{r}_\alpha\})$$

**Transformed Lagrangian:**

$$\begin{aligned} L'(\{\mathbf{r}'_\alpha, \dot{\mathbf{r}}'_\alpha\}) &= T' - U' \\ &= \sum_{\alpha=1}^N \frac{m_\alpha}{2} \dot{\mathbf{r}}_\alpha \cdot \dot{\mathbf{r}}_\alpha + \sum_{\alpha=1}^N m_\alpha \dot{\mathbf{r}}_\alpha \cdot \mathbf{V} + \sum_{\alpha=1}^N \frac{m_\alpha}{2} \mathbf{V} \cdot \mathbf{V} - U \\ &= L(\{\mathbf{r}_\alpha, \dot{\mathbf{r}}_\alpha\}) + \sum_{\alpha=1}^N m_\alpha \dot{\mathbf{r}}_\alpha \cdot \mathbf{V} + \sum_{\alpha=1}^N \frac{m_\alpha}{2} \mathbf{V} \cdot \mathbf{V} \end{aligned}$$

**Express in primed coordinates:**

Since  $\dot{\mathbf{r}}_\alpha = \dot{\mathbf{r}}'_\alpha - \mathbf{V}$  and  $\mathbf{r}_\alpha = \mathbf{r}'_\alpha - \mathbf{V}t$ :

$$L'(\{\mathbf{r}'_\alpha, \dot{\mathbf{r}}'_\alpha\}) = L(\{\mathbf{r}'_\alpha, \dot{\mathbf{r}}'_\alpha\}) + \sum_{\alpha=1}^N m_\alpha \dot{\mathbf{r}}'_\alpha \cdot \mathbf{V} - \sum_{\alpha=1}^N m_\alpha \mathbf{V} \cdot \mathbf{V} + \sum_{\alpha=1}^N \frac{m_\alpha}{2} \mathbf{V} \cdot \mathbf{V}$$

$$L'(\{\mathbf{r}'_\alpha, \dot{\mathbf{r}}'_\alpha\}) = L(\{\mathbf{r}'_\alpha, \dot{\mathbf{r}}'_\alpha\}) + \sum_{\alpha=1}^N m_\alpha \dot{\mathbf{r}}'_\alpha \cdot \mathbf{V} - \sum_{\alpha=1}^N \frac{m_\alpha}{2} \mathbf{V} \cdot \mathbf{V}$$

**Identify as gauge transformation:**

A gauge transformation has the form:

$$L' = L + \frac{d\Lambda}{dt}$$

where  $\Lambda$  is the gauge function. We need:

$$\frac{d\Lambda}{dt} = \sum_{\alpha=1}^N m_\alpha \dot{\mathbf{r}}'_\alpha \cdot \mathbf{V} - \sum_{\alpha=1}^N \frac{m_\alpha}{2} \mathbf{V} \cdot \mathbf{V}$$

Rewriting:

$$\frac{d\Lambda}{dt} = - \sum_{\alpha=1}^N m_\alpha \mathbf{V} \cdot \dot{\mathbf{r}}'_\alpha + \sum_{\alpha=1}^N \frac{m_\alpha}{2} \mathbf{V} \cdot \mathbf{V}$$

**Integrate to find gauge function:**

$$\frac{d\Lambda}{dt} = -\mathbf{V} \cdot \frac{d}{dt} \left[ \sum_{\alpha=1}^N m_\alpha \mathbf{r}'_\alpha \right] + \sum_{\alpha=1}^N \frac{m_\alpha}{2} \mathbf{V} \cdot \mathbf{V}$$

Integrating:

$$\Lambda = -\mathbf{V} \cdot \sum_{\alpha=1}^N m_\alpha \mathbf{r}'_\alpha + \sum_{\alpha=1}^N \frac{m_\alpha}{2} (\mathbf{V} \cdot \mathbf{V}) t + \text{const}$$

Alternatively, dropping the constant and primes:

$$\Lambda(\{\mathbf{r}_\alpha\}, t) = - \sum_{\alpha=1}^N m_\alpha \mathbf{r}_\alpha \cdot \mathbf{V} + \frac{1}{2} \left( \sum_{\alpha=1}^N m_\alpha \right) |\mathbf{V}|^2 t$$

**Conclusion:** The Galilean transformation is indeed a gauge transformation, meaning that both Lagrangians give the same equations of motion, as they must for physical consistency (the laws of physics are the same in all inertial frames).

**Problem 9.1**

Starting from  $g = g(u, y)$ , perform a Legendre transformation to another function  $h = h(x, v)$ .

**Given:**  $f = f(x, y)$  with  $df = u dx + v dy$

**First transformation ( $f \rightarrow g$ ):**

$$u = \frac{\partial f}{\partial x_y} \Rightarrow x = x(u, y)$$

$$g(u, y) \equiv f(x(u, y), y) - x(u, y)u$$

$$dg = -x du + v dy$$

**Solution**

**Starting point:**

We have  $g = g(u, y)$  with differential:

$$dg = -x du + v dy$$

From this differential, we identify:

$$\begin{cases} x = -\frac{\partial g}{\partial u_y} \\ v = \frac{\partial g}{\partial y_u} \end{cases}$$

**Choose new independent variables:**

We want to transform from  $(u, y)$  to  $(x, v)$ . This requires:

- $u$  should become a dependent variable (function of  $x$  and  $v$ )
- $y$  should become a dependent variable (function of  $x$  and  $v$ )

This means we need to perform two Legendre transformations: one to change  $u \rightarrow x$  and another to change  $y \rightarrow v$ .

**Legendre transformation to change both variables:**

The Legendre transformation from  $g(u, y)$  to  $h(x, v)$  is:

$$h(x, v) \equiv g(u(x, v), y(x, v)) + u(x, v)x - y(x, v)v$$

**Calculate the differential of  $h$ :**

Taking the total differential:

$$dh = dg + (u dx + x du) - (y dv + v dy)$$

Substituting  $dg = -x du + v dy$ :

$$dh = (-x du + v dy) + (u dx + x du) - (y dv + v dy)$$

$$dh = u dx - y dv$$

**Identify partial derivatives:**

From  $dh = u dx - y dv$ , we have:

$$\begin{cases} u = \frac{\partial h}{\partial x_v} \\ -y = \frac{\partial h}{\partial v_x} \end{cases} \Rightarrow y = -\frac{\partial h}{\partial v_x}$$

**Summary of transformations:**

Starting from  $f(x, y)$  with  $df = u \, dx + v \, dy$ :

$$\begin{cases} \text{First:} & g(u, y) = f - ux, & dg = -x \, du + v \, dy \\ \text{Second:} & h(x, v) = g + ux - vy, & dh = u \, dx - y \, dv \end{cases}$$

Combining the two transformations:

$$h(x, v) = [f - ux] + ux - vy = f - vy$$

$$h(x, v) = f(x, y(x, v)) - vy(x, v)$$

with differential  $dh = u \, dx - y \, dv$ .

**Alternative formulation:**

We could also write:

$$h(x, v) = -[vy - f(x, y)]$$

or in terms of  $g$ :

$$h(x, v) = g(u(x, v), y(x, v)) + u(x, v)x - y(x, v)v$$

**Verification:**

$$\begin{aligned} dh &= \frac{\partial g}{\partial u_y} \, du + \frac{\partial g}{\partial y_u} \, dy + u \, dx + x \, du - y \, dv - v \, dy \\ &= -x \, du + v \, dy + u \, dx + x \, du - y \, dv - v \, dy \\ &= u \, dx - y \, dv \quad \checkmark \end{aligned}$$